AE and DH go through, PKAE still WIP

secure_api/box/Box.DH.fst
@@ -1,6 +1,5 @@
 (**
    TODO: - Documentation, some cleanup.
-	 - make decrypt a total function.
 *)
 module Box.DH
 
@@ -13,24 +12,30 @@ open FStar.Monotonic.Seq
 open FStar.List.Tot
 
 open CoreCrypto
-open Platform.Bytes
 
 open Box.Indexing
-open Box.PlainDH
 open Box.Flags
 
 module MR = FStar.Monotonic.RRef
 module MM = MonotoneMap
 module HS = FStar.HyperStack
 module HH = FStar.HyperHeap
+module HSalsa = Spec.HSalsa20
+module Curve = Spec.Curve25519
+module Key = Box.AE.Key
 
-
-assume val dh_element_size : nat
-assume val dh_exponent_size : nat
-type dh_element =lbytes dh_element_size
-type dh_share = dh_element
+#set-options "--z3rlimit 100 --lax"
+let dh_element_size = HSalsa.keylen // is equal to scalar lenght in Spec.Curve25519
+let dh_exponent_size = 32 //TODO: replace with constant from Spec.Curve25519
+type dh_element = HSalsa.key
+type dh_share = Curve.serialized_point //
 assume val dh_base : dh_element
-abstract type dh_exponent = lbytes dh_exponent_size
+type dh_exponent = Curve.scalar // is equal to Curve.serialized_point
+
+(**
+   Nonce to use with HSalsa.hsalsa20.
+*)
+private let zero_nonce = Seq.create HSalsa.noncelen (UInt8.uint_to_t 0)
 
 assume val dh_gen_key: unit -> ST (dh_share*dh_exponent)
   (requires (fun h0 -> True))
@@ -38,49 +43,80 @@ assume val dh_gen_key: unit -> ST (dh_share*dh_exponent)
     h0==h1
   ))
 
-type aes_key = PlainDH.aes_key 
-assume val hash: dh_element -> Tot aes_key
-
-(*
-  Setting up a global log for AE.keys indexed by the ids of the public and private key involved.
-*)
-private type dh_key_log_range = fun (k_id:id{AE_id? k_id}) -> k:PlainDH.key{PlainDH.ae_key_get_index k = k_id}
-
-(**
-   Invariant for the dh_key_log: If a key is honest and we idealize prf_odh, then if it is unfresh,
-   there has to be an entry in the dh_key_log.
-*)
-private let dh_key_log_inv (m:MM.map' (i:id{AE_id? i}) dh_key_log_range) = True
-//  forall (i:id{AE_id? i}). (honest i /\ prf_odh) ==> (Some? (MM.sel m i) ==> unfresh i)
+type aes_key = Key.aes_key 
 
 
 assume val dh_key_log_region: (r:HH.rid{ extends r root 
 					 /\ is_eternal_region r 
 					 /\ is_below r root 
-					 /\ disjoint r ae_key_region
-					 /\ disjoint r id_freshness_table_region
-					 /\ disjoint r id_honesty_table_region
+					 /\ disjoint r Key.ae_key_region
+					 /\ disjoint r id_log_region
+					 /\ disjoint r id_honesty_log_region
 					 })
+
+//private type dh_key_log_key = k_id:id{AE_id? k_id}
+//private type dh_key_log_value = 
+private type dh_key_log_range = fun (k_id:id{AE_id? k_id}) -> (k:Key.key{Key.ae_key_get_index k = k_id})
+private let dh_key_log_inv (m:MM.map' (k_id:id{AE_id? k_id}) dh_key_log_range) = True
+
+(**
+   The dh_key_log is a monotone map that maps ids to AE keys. Keys that are generated/computed by prf_odh are random if both DH keys
+   that serve as its input are honest. Such honest keys are stored in the dh_key_log to ensure that only one AE key is generated for each
+   pair of DH keys. This is ensured by the monotone nature of the log and the composition of AE ids through DH ids.
+*)
 assume val dh_key_log: MM.t dh_key_log_region (i:id{AE_id? i}) dh_key_log_range dh_key_log_inv
 
-noeq abstract type dh_pkey = 
+(**
+   A DH public key containing its raw byte representation. All ids of DH keys have to be unfresh and registered (e.g. marked as either honest
+   or dishonest).
+   TODO: Does the public key have to be abstract?
+*)
+noeq type dh_pkey = 
   | DH_pkey: #pk_id:id{DH_id? pk_id /\ unfresh pk_id /\ registered pk_id} -> rawpk:dh_share -> dh_pkey
 
+(**
+   A DH secret key containing its raw byte representation. All ids of DH keys have to be unfresh and registered (e.g. marked as either honest
+   or dishonest).
+*)
 noeq abstract type dh_skey =
   | DH_skey: #sk_id:id{DH_id? sk_id /\ unfresh sk_id /\ registered sk_id} -> rawsk:dh_exponent -> pk:dh_pkey{pk.pk_id=sk_id} -> dh_skey 
 
+(**
+   A helper function to obtain the index of a DH secret key.
+*)
 val sk_get_index: sk:dh_skey -> Tot (i:id{i = sk.sk_id})
 let sk_get_index k = k.sk_id
 
+(**
+   A helper function to obtain the index of a DH public key.
+*)
 val pk_get_index: pk:dh_pkey -> Tot (i:id{i = pk.pk_id})
 let pk_get_index k = k.pk_id
 
+
+val get_skey: sk:dh_skey -> GTot (raw:dh_exponent{raw=sk.rawsk})
+let get_skey sk = 
+  sk.rawsk
+
+(**
+   This function provides access to the raw byte representation of a DH public key.
+   TODO: If the key is not abstract, we do not need this any longer.
+*)
 val pk_get_rawpk: pk:dh_pkey -> Tot (raw:dh_share{raw=pk.rawpk})
 let pk_get_rawpk pk =
   pk.rawpk
 
+val leak_skey: sk:dh_skey{dishonest sk.sk_id} -> Tot (raw:dh_exponent{raw=sk.rawsk})
+let leak_skey sk = 
+  sk.rawsk
+
+// TODO: Replace this with curve25519 scalar multiplication.
 assume val dh_exponentiate: dh_element -> dh_exponent -> Tot dh_element
 
+(**
+   keygen generates a pair of DH keys with the same id. It requires that the id associated with the keys
+   is registered. The id is considered unfresh after key generation.
+*)
 val keygen: #i:id{DH_id? i} -> ST (dh_pair:(k:dh_pkey{k.pk_id=i}) * (k:dh_skey{k.sk_id=i}))
   (requires (fun h -> 
     fresh i h
@@ -88,7 +124,7 @@ val keygen: #i:id{DH_id? i} -> ST (dh_pair:(k:dh_pkey{k.pk_id=i}) * (k:dh_skey{k
   ))
   (ensures (fun h0 k h1 -> 
     unfresh i
-    /\ modifies (Set.singleton id_freshness_table_region) h0 h1
+    /\ modifies (Set.singleton id_log_region) h0 h1
   ))
 let keygen #i =
   make_unfresh i;
@@ -97,6 +133,10 @@ let keygen #i =
   let dh_sk = DH_skey #i dh_exponent dh_pk in
   dh_pk,dh_sk
 
+(**
+   coerce_pkey allows the adversary to coerce any DH share into a DH public key. Such a coerced key has
+   to be dishonest. Also, the id is considered unfresh after coercion.
+*)
 val coerce_pkey: #i:id{DH_id? i /\ dishonest i} -> dh_share -> ST (pk:dh_pkey{pk.pk_id=i})
   (requires (fun h0 -> 
     fresh i h0
@@ -108,7 +148,10 @@ val coerce_pkey: #i:id{DH_id? i /\ dishonest i} -> dh_share -> ST (pk:dh_pkey{pk
 let coerce_pkey #i dh_sh =
   make_unfresh i;
   DH_pkey #i dh_sh
-
+(**
+   coerce_keypair allows the adversary to coerce a DH exponent into a DH private key. The corresponding DH public key
+   is generated along with it. Both keys are considered dishonest and the id is considered unfresh after coercion.
+*)
 val coerce_keypair: #i:id{DH_id? i /\ dishonest i} -> dh_exponent -> ST (dh_pair:(k:dh_pkey{k.pk_id=i}) * (k:dh_skey{k.sk_id=i}))
   (requires (fun h0 -> 
     fresh i h0
@@ -124,71 +167,146 @@ let coerce_keypair #i dh_ex =
   let sk = DH_skey #i dh_ex pk in
   pk,sk
 
-
-// Make this function GTot
-val prf_odhT: dh_skey -> dh_pkey -> GTot aes_key
-let prf_odhT dh_sk dh_pk =
+(**
+   GTot specification of the prf_odh function for use in type refinements.
+*)
+val prf_odhGT: dh_skey -> dh_pkey -> GTot aes_key
+let prf_odhGT dh_sk dh_pk =
   let pk_id = dh_pk.pk_id in
   let sk_id = dh_sk.sk_id in
   let i = generate_ae_id pk_id sk_id in
-  let raw_k = dh_exponentiate dh_pk.rawpk dh_sk.rawsk in
-  let k = hash raw_k in
+  let raw_k = Curve.scalarmult dh_sk.rawsk dh_pk.rawpk in
+  let k = HSalsa.hsalsa20 raw_k zero_nonce in
   k
 
-#set-options "--z3rlimit 25"
-val prf_odh: sk:dh_skey -> pk:dh_pkey -> ST (PlainDH.key)
+
+#reset-options
+#set-options "--z3rlimit 100"
+val handle_honest_i: i:id{AE_id? i /\ honest i} -> ST (k:Key.key)
+  (requires (fun h0 -> 
+    ((AE_id? i /\ honest i) ==> (MM.defined dh_key_log i h0 \/ fresh i h0))
+  ))
+  (ensures (fun h0 k h1 ->
+    let regions_modified_honest = Set.union (Set.singleton id_log_region) (Set.singleton dh_key_log_region) in
+    let k_log = Key.get_logGT k in
+    let current_log = MR.m_sel h0 dh_key_log in
+    i = Key.ae_key_get_index k
+    /\ MR.m_contains k_log h1
+    /\ (fresh i h0 ==> (MR.m_sel h1 (Key.get_logGT k) == Key.empty_log i))
+    /\ MR.witnessed (MM.contains dh_key_log i k)
+    /\ (MM.fresh dh_key_log i h0 ==> (MR.m_sel h1 dh_key_log == MM.upd current_log i k // if the key is not yet in the dh_key_log, it will be afterwards
+    			          /\ MR.m_sel h1 k_log == Key.empty_log i     // and the log of the key will be empty.
+    				  /\ makes_unfresh_just i h0 h1))
+    /\ (MM.defined dh_key_log i h0 ==> (MR.m_sel h0 dh_key_log == MR.m_sel h1 dh_key_log // if the key is in the dh_key_log, the dh_key_log will not be modified
+    			            /\ MR.m_sel h0 k_log == MR.m_sel h1 k_log))       // and the log of the key will be the same as before.
+    /\ HS.modifies regions_modified_honest h0 h1
+  ))
+let handle_honest_i i = 
+  //lemma_honest_not_dishonest i;
+  MR.m_recall dh_key_log;
+  match MM.lookup dh_key_log i with
+  | Some  k' ->
+    Key.recall_log k'; 
+    MR.m_recall id_log;
+    fresh_unfresh_contradiction i;
+    k'
+  | None ->
+    let h0 = ST.get() in
+    let k' = Key.keygen i in
+    MR.m_recall dh_key_log;
+    MR.m_recall id_log;
+    MM.extend dh_key_log i k';
+    Key.recall_log k';
+    fresh_unfresh_contradiction i;
+    k'
+
+#reset-options
+#set-options "--z3rlimit 100"
+val handle_dishonest_i:  dh_sk:dh_skey 
+		       -> dh_pk:dh_pkey 
+		       -> i:id{dishonest i /\ AE_id? i /\ i = generate_ae_id dh_pk.pk_id dh_sk.sk_id} 
+		       -> ST (k:Key.key{Key.ae_key_get_index k = i})
+  (requires (fun h0 -> registered i))
+  (ensures (fun h0 k h1 -> 
+    let regions_modified_dishonest:Set.set (r:HH.rid) = (Set.singleton id_log_region) in
+    let k_log = Key.get_logGT k in
+    HS.modifies regions_modified_dishonest h0 h1
+    /\ Key.leak_key k = prf_odhGT dh_sk dh_pk
+    /\ MR.m_contains k_log h1
+    /\ makes_unfresh_just i h0 h1
+    /\ i = Key.ae_key_get_index k 
+    /\ MR.m_sel h1 (Key.get_logGT k) == Key.empty_log i
+  ))
+let handle_dishonest_i dh_sk dh_pk i =
+    lemma_dishonest_not_honest i;
+    let raw_k = Curve.scalarmult dh_sk.rawsk dh_pk.rawpk in
+    let hashed_raw_k = HSalsa.hsalsa20 raw_k zero_nonce in
+    let k=Key.coerce_key i hashed_raw_k in
+    fresh_unfresh_contradiction i;
+    k
+
+
+// This everifies now. Inlining handler functions for honest and dishonest case breaks things...
+val prf_odh: sk:dh_skey -> pk:dh_pkey -> ST (Key.key)
   ( requires (fun h0 -> 
     let i = generate_ae_id pk.pk_id sk.sk_id in
     ((AE_id? i /\ honest i) ==> (MM.defined dh_key_log i h0 \/ fresh i h0))
-    /\ m_contains id_freshness_table h0
+    /\ m_contains id_log h0
+    /\ registered i
   ))
   ( ensures (fun h0 k h1 ->
     let i = generate_ae_id pk.pk_id sk.sk_id in
-    let regions_modified_dishonest:Set.set (r:HH.rid) = (Set.singleton id_freshness_table_region) in
+    let regions_modified_dishonest:Set.set (r:HH.rid) = (Set.singleton id_log_region) in
     let regions_modified_honest = Set.union regions_modified_dishonest (Set.singleton dh_key_log_region) in
-    let k_log = get_logGT k in
-    (PlainDH.ae_key_get_index k = i)
+    let k_log = Key.get_logGT k in
+    (i = Key.ae_key_get_index k)
     /\ MR.m_contains k_log h1
-    /\ (fresh i h0 ==> (MR.m_sel h1 (PlainDH.get_logGT k) == PlainDH.empty_log i))
+    /\ (fresh i h0 ==> (MR.m_sel h1 (Key.get_logGT k) == Key.empty_log i))
     /\ (honest i ==> (let current_log = MR.m_sel h0 dh_key_log in
-		   MR.witnessed (MM.contains dh_key_log i k)
-		   /\ (MM.fresh dh_key_log i h0 ==> (MR.m_sel h1 dh_key_log == MM.upd current_log i k // if the key is not yet in the dh_key_log, it will be afterwards
-						  /\ MR.m_sel h1 k_log == PlainDH.empty_log i))     // and the log of the key will be empty.
-		   /\ (MM.defined dh_key_log i h0 ==> (MR.m_sel h0 dh_key_log == MR.m_sel h1 dh_key_log // if the key is in the dh_key_log, the dh_key_log will not be modified
-						    /\ MR.m_sel h0 k_log == MR.m_sel h1 k_log))       // and the log of the key will be the same as before.
-		   /\ modifies regions_modified_honest h0 h1
-		  )
-      )
+    		   MR.witnessed (MM.contains dh_key_log i k)
+    		   /\ (MM.fresh dh_key_log i h0 ==> (MR.m_sel h1 dh_key_log == MM.upd current_log i k // if the key is not yet in the dh_key_log, it will be afterwards
+    						  /\ MR.m_sel h1 k_log == Key.empty_log i // and the log of the key will be empty.
+						  /\ makes_unfresh_just i h0 h1))
+    		   /\ (MM.defined dh_key_log i h0 ==> (MR.m_sel h0 dh_key_log == MR.m_sel h1 dh_key_log // if the key is in the dh_key_log, the dh_key_log will not be modified
+    						    /\ MR.m_sel h0 k_log == MR.m_sel h1 k_log))       // and the log of the key will be the same as before.
+    		   /\ modifies regions_modified_honest h0 h1))
     /\ (dishonest i
     	==> (modifies regions_modified_dishonest h0 h1
-    	   /\ leak_key k = prf_odhT sk pk
-    	  )
-      )
-    /\ makes_unfresh_just i h0 h1
+    	   /\ Key.leak_key k = prf_odhGT sk pk
+	   /\ makes_unfresh_just i h0 h1))
   ))
 let prf_odh dh_sk dh_pk =
+  let h0 = ST.get() in
   let i = generate_ae_id dh_pk.pk_id dh_sk.sk_id in
   let honest_i = is_honest i in
   MR.m_recall dh_key_log;
+  MR.m_recall id_log;
+  MR.m_recall id_honesty_log;
   if honest_i then (
+    // This branch checks out!
     lemma_honest_not_dishonest i;
-    MR.m_recall dh_key_log;
-    match MM.lookup dh_key_log i with
-    | Some  k' ->
-	recall_log k'; 
-	fresh_unfresh_contradiction i;
-        k'
-    | None ->
-        let k' = PlainDH.keygen i in
-        MM.extend dh_key_log i k';
-	fresh_unfresh_contradiction i;
-        k'
+    let k = handle_honest_i i in
+    k
+//    MR.m_recall dh_key_log;
+//    match MM.lookup dh_key_log i with
+//    | Some  k' ->
+//	Key.recall_log k'; 
+//	fresh_unfresh_contradiction i;
+//        k'
+//    | None ->
+//        let k' = Key.keygen i in
+//        MM.extend dh_key_log i k';
+//	fresh_unfresh_contradiction i;
+//        k'
   ) else (
+    // Getting an "unknown assertion failed" error in this branch
     lemma_dishonest_not_honest i;
-    let raw_k = dh_exponentiate dh_pk.rawpk dh_sk.rawsk in
-    let hashed_raw_k = hash raw_k in
-    let k=PlainDH.coerce_key i hashed_raw_k in
-    fresh_unfresh_contradiction i;
-    k)
+    let k = handle_dishonest_i dh_sk dh_pk i in
+    k
+//    let raw_k = Curve.scalarmult dh_sk.rawsk dh_pk.rawpk in
+//    let hashed_raw_k = HSalsa.hsalsa20 raw_k zero_nonce in
+//    let k=Key.coerce_key i hashed_raw_k in
+//    fresh_unfresh_contradiction i;
+//    k
+  )
 
-#reset-options
